list Vectors retS and cases

list_vector/ListVectorDef.v
@@ -21,6 +21,96 @@ Definition cons (A : Type) (h : A) (n : nat) (v : t A n) : t A (S n) :=
 Local Notation "[ ]" := (nil _) (format "[ ]").
 Local Notation "h :: t" := (cons _ h _ t) (at level 60, right associativity).
 
+Require Import Lia.
+
+Lemma vec_spec_eq: forall {A:Type} {n:nat}, forall (v1 v2: t A n), elts v1 = elts v2 <-> v1 = v2.
+Proof.
+intros.
+split.
+- intros H.
+  destruct v1, v2.
+  cbn in *.
+  destruct H.
+  enough (elts_spec0 = elts_spec1).
+  + rewrite H.
+    reflexivity.
+  + Check Eqdep_dec.UIP_dec.
+    apply Eqdep_dec.UIP_dec.
+    apply PeanoNat.Nat.eq_dec.
+- intros H.
+  destruct v1, v2.
+  apply (f_equal elts) in H.
+  cbn in *.
+  apply H.
+Qed.
+
+
+Definition rectS {A} (P:forall {n}, t A (S n) -> Type)
+(bas: forall a: A, P (a :: []))
+(rect: forall a {n} (v: t A (S n)), P v -> P (a :: v)) 
+: forall (n:nat) (v:t A (S n)), P v.
+Proof.
+refine (fix rectS_fix (n:nat) (v:t A (S n)) : @P n v := _).
+destruct v.
+destruct elts0.
+- refine (match lia_utils.S_not_0 n elts_spec0 with end).
+- destruct elts0.
+  + apply (f_equal pred) in elts_spec0 as H.
+    cbn in H.
+    destruct H.
+    rewrite (lia_utils.nat_uip elts_spec0 eq_refl).
+    refine (bas a).
+  + destruct n.
+    * apply (f_equal pred) in elts_spec0 as H.
+      refine (match lia_utils.S_not_0 _ (eq_sym H) with end).
+    * apply (f_equal pred) in elts_spec0 as H.
+      change (Init.Nat.pred (length (a :: a0 :: elts0)) = Init.Nat.pred (S (S n))) with (length (a0::elts0) = S n) in H.
+      specialize (rect a n {|elts := a0 :: elts0; elts_spec := H|}).
+      specialize (rectS_fix n {| elts := a0 :: elts0; elts_spec := H |}).
+      specialize (rect rectS_fix).
+      unfold cons in rect.
+      cbn in rect.
+      rewrite (lia_utils.nat_uip elts_spec0 (f_equal S H)).
+      refine (rect).
+Defined.
+
+Definition case0 {A} (P:t A 0 -> Type) (H:P (nil A)) v:P v:=
+match v with | {| elts := l; elts_spec := l_sp |} => 
+  match l return (forall l_sp, P {| elts := l; elts_spec := l_sp |}) with
+  | Datatypes.nil => fun l_sp => 
+    rew <- [fun l_sp => P {| elts := Datatypes.nil; elts_spec := l_sp |}] nat_uip l_sp eq_refl in H
+  | (a :: l)%list => fun l_sp => match S_not_0 _ (eq_sym l_sp) with end
+  end l_sp
+end.
+
+Definition caseS {A} (P : forall {n}, t A (S n) -> Type)
+  (H : forall h {n} t, @P n (h :: t)) {n} (v: t A (S n)) : P v :=
+match v with {| elts := l; elts_spec := l_sp |} => 
+    match l return (forall l_sp : length l = S n, P {| elts := l; elts_spec := l_sp |}) with
+    | Datatypes.nil => fun l_sp => match S_not_0 n l_sp with end
+    | (a :: l)%list => fun l_sp => 
+          rew [fun e => P {| elts := a :: l; elts_spec := e |}] nat_uip (f_equal S (f_equal pred l_sp)) l_sp in 
+          H a {| elts := l; elts_spec := f_equal pred l_sp |}
+    end l_sp
+end.
+  
+Definition caseS' {A} {n : nat} (v : t A (S n)) : forall (P : t A (S n) -> Type)
+(H : forall h t, P (h :: t)), P v :=
+match v with
+| h :: t => fun P H => H h t
+| _ => fun devil => False_rect (@IDProp) devil
+end.
+
+Definition rect2 {A B} (P:forall {n}, t A n -> t B n -> Type)
+(bas : P [] []) (rect : forall {n v1 v2}, P v1 v2 ->
+  forall a b, P (a :: v1) (b :: v2)) :=
+fix rect2_fix {n} (v1 : t A n) : forall v2 : t B n, P v1 v2 :=
+match v1 with
+| [] => fun v2 => case0 _ bas v2
+| @cons _ h1 n' t1 => fun v2 =>
+  caseS' v2 (fun v2' => P (h1::t1) v2') (fun h2 t2 => rect (rect2_fix t1 t2) h1 h2)
+end.
+
 Lemma vector_ind : forall (A : Type) (P : forall n : nat, t A n -> Prop),
   P 0 (nil _) -> (forall (h : A) (n : nat) (v : t A n), P n v -> P (S n) (cons _ h n v)) ->
   forall (n : nat) (v : t A n), P n v.
